src/Appraisal_AltImpls_Eq.v
@@ -1,0 +1,403 @@
+Require Import Maps Event_system Term_system MonadVM ConcreteEvidence.
+Require Import Impl_vm Helpers_VmSemantics VmSemantics.
+Require Import Axioms_Io External_Facts Auto AutoApp.
+
+Require Import StAM Appraisal_Defs Impl_appraisal (*MonadAM*).
+
+Require Import Coq.Arith.Peano_dec.
+
+Require Import StructTactics OptMonad.
+
+Require Import Coq.Program.Tactics Coq.Program.Equality.
+
+Require Import List.
+Import ListNotations.
+
+Require Import Lia.
+
+Require Import Impl_appraisal_alt.
+
+Set Nested Proofs Allowed.
+
+
+Check Impl_appraisal_alt.build_app_comp_evC.
+Check Impl_appraisal.build_app_comp_evC.
+
+Lemma inv_recon_mt: forall ls et,
+    reconstruct_ev' ls et = Some mtc ->
+    et = mt.
+Proof.
+  intros.
+  destruct et; repeat ff; try solve_by_inversion.
+Defined.
+
+Lemma inv_recon_nn: forall ls et n n0,
+    reconstruct_ev' ls et = Some (nnc n n0) ->
+    et = nn n.
+Proof.
+  intros.
+  destruct et; repeat ff; try solve_by_inversion.
+Defined.
+
+Lemma inv_recon_uu: forall ls et n l n0 n1 n2 ec,
+    reconstruct_ev' ls et = Some (uuc n l n0 n1 n2 ec) ->
+    (exists et', et = uu n l n0 n1 et').
+Proof.
+  intros.
+  destruct et; repeat ff; try solve_by_inversion.
+  eauto.
+Defined.
+
+Lemma inv_recon_gg: forall ls et n n0 ec,
+    reconstruct_ev' ls et = Some (ggc n n0 ec) ->
+    (exists et', et = gg n et').
+Proof.
+  intros.
+  destruct et; repeat ff; try solve_by_inversion.
+  eauto.
+Defined.
+
+Lemma inv_recon_hh: forall ls et n n0 et',
+    reconstruct_ev' ls et = Some (hhc n n0 et') ->
+    (et = hh n et' ).
+Proof.
+  intros.
+  destruct et; repeat ff; try solve_by_inversion.
+Defined.
+
+Lemma inv_recon_ss: forall ls et ec1 ec2,
+    reconstruct_ev' ls et = Some (ssc ec1 ec2) ->
+    (exists et1 et2, et = ss et1 et2).
+Proof.
+  intros.
+  destruct et; repeat ff; try solve_by_inversion.
+  eauto.
+Defined.
+
+Lemma inv_recon_pp: forall ls et ec1 ec2,
+    reconstruct_ev' ls et = Some (ppc ec1 ec2) ->
+    (exists et1 et2, et = pp et1 et2).
+Proof.
+  intros.
+  destruct et; repeat ff; try solve_by_inversion.
+  eauto.
+Defined.
+
+Lemma recon_encodeEv : forall ls et ec,
+    wf_ec (evc ls et) -> 
+    reconstruct_ev' ls et = Some ec ->
+    ls = encodeEv ec.
+Proof.
+  intros.
+  generalizeEverythingElse ec.
+  induction ec; intros.
+  -
+    ff.
+    assert (et = mt).
+    {
+      eapply inv_recon_mt; eauto.
+    }
+    subst.
+    invc H.
+    ff.
+    destruct ls; try solve_by_inversion.
+  (* TODO: exclude mt case? *)
+  -
+    ff.
+    assert (et = nn n).
+    {
+      eapply inv_recon_nn; eauto.
+    }
+    subst.
+    repeat ff.
+    destruct ls; try solve_by_inversion.
+    invc H.
+    ff.
+    assert (e = []).
+    destruct e; try solve_by_inversion.
+    ff.
+  -
+    ff.
+    assert (exists et', et = uu n l n0 n1 et').
+    {
+      eapply inv_recon_uu; eauto.
+    }
+    destruct_conjs.
+    subst.
+    repeat ff.
+    invc H.
+    ff.
+    edestruct IHec with (ls := e).
+    2: {
+      eassumption.
+    }
+    econstructor.
+    destruct ls; try solve_by_inversion.
+    unfold peel_bs in *.
+    ff.
+  -
+    ff.
+    assert (exists et', et = gg n et').
+    {
+      eapply inv_recon_gg; eauto.
+    }
+    destruct_conjs.
+    subst.
+    repeat ff.
+    invc H.
+    ff.
+    edestruct IHec with (ls := e).
+    2: {
+      eassumption.
+    }
+    econstructor.
+    destruct ls; try solve_by_inversion.
+    unfold peel_bs in *.
+    ff.
+  -
+    ff.
+    assert (et = hh n e).
+    {
+      eapply inv_recon_hh; eauto.
+    }
+    subst.
+    repeat ff.
+    invc H.
+    ff.
+    destruct ls; try solve_by_inversion.
+    ff.
+    assert (e0 = []).
+    { destruct e0; try solve_by_inversion. }
+    subst.
+    ff.
+  -
+    ff.
+    assert (exists et1 et2, et = ss et1 et2).
+    {
+      eapply inv_recon_ss; eauto.
+    }
+    destruct_conjs.
+    subst.
+    repeat ff.
+    invc H.
+    ff.
+
+    assert ((firstn (et_size H1) ls) = encodeEv ec1).
+    { eapply IHec1 with (et:= H1).
+      econstructor.
+      eapply firstn_long.
+      lia.
+      eassumption.
+    }
+
+    assert ((skipn (et_size H1) ls) = encodeEv ec2).
+    {
+      eapply IHec2 with (et := H2).
+      econstructor.
+      eapply skipn_long.
+      lia.
+      eassumption.
+    }
+    jkjke'.
+    jkjke'.
+    Search firstn.
+    rewrite firstn_skipn.
+    tauto.
+    -
+      ff.
+    assert (exists et1 et2, et = pp et1 et2).
+    {
+      eapply inv_recon_pp; eauto.
+    }
+    destruct_conjs.
+    subst.
+    repeat ff.
+    invc H.
+    ff.
+
+    assert ((firstn (et_size H1) ls) = encodeEv ec1).
+    { eapply IHec1 with (et:= H1).
+      econstructor.
+      eapply firstn_long.
+      lia.
+      eassumption.
+    }
+
+    assert ((skipn (et_size H1) ls) = encodeEv ec2).
+    {
+      eapply IHec2 with (et := H2).
+      econstructor.
+      eapply skipn_long.
+      lia.
+      eassumption.
+    }
+    jkjke'.
+    jkjke'.
+    Search firstn.
+    rewrite firstn_skipn.
+    tauto.
+Defined.
+
+
+Lemma appraisal_alt : forall ec1 ec2 ec2' ls et,
+
+  Some ec1 = Impl_appraisal_alt.build_app_comp_evC et ls ->
+  Some ec2 = Impl_appraisal.reconstruct_ev (evc ls et) ->
+  ec2' = Impl_appraisal.build_app_comp_evC ec2 ->
+  ec1 = ec2'.
+Proof.
+  intros.
+  generalizeEverythingElse ec2.
+  induction ec2; intros.
+  -
+    ff.
+    subst.
+    assert (et = mt).
+    { eapply inv_recon_mt; eauto. }
+    subst.
+    ff.
+  -
+    ff.
+    subst.
+    assert (et = nn n).
+    { eapply inv_recon_nn; eauto. }
+    subst.
+    repeat ff.
+  -
+    ff.
+    subst.
+    ff.
+    assert (exists et', et = uu n l n0 n1 et').
+    { eapply inv_recon_uu; eauto. }
+    destruct_conjs.
+    subst.
+    repeat ff.
+
+    (*
+
+    assert (Impl_appraisal.peel_bs = peel_bs) as H.
+    { admit. }
+    rewrite H in *; clear H. 
+    find_rewrite.
+    ff. *)
+
+    assert (e0 = (Impl_appraisal.build_app_comp_evC e1)).
+    {
+      eapply IHec2.
+      jkjke.
+      jkjke.
+      tauto.
+    }
+    subst.
+    congruence.
+  -
+    ff.
+    subst.
+    ff.
+    assert (exists et', et = gg n et').
+    { eapply inv_recon_gg; eauto. }
+    destruct_conjs.
+    subst.
+    repeat ff.
+
+    (*
+
+    assert (Impl_appraisal.peel_bs = peel_bs) as H.
+    { admit. }
+    rewrite H in *; clear H. 
+    find_rewrite.
+    ff. *)
+
+    assert (e0 = (Impl_appraisal.build_app_comp_evC e1)).
+    {
+      eapply IHec2.
+      jkjke.
+      jkjke.
+      tauto.
+    }
+    subst.
+    unfold checkSig.
+    assert (checkSigBits e n n1 =
+            checkSigBits (encodeEv e1) n n1).
+    {
+      assert (e = encodeEv e1).
+      {
+        eapply recon_encodeEv.
+        2: { eassumption. }
+
+        Lemma wf_recon: forall e et ec,
+          reconstruct_ev' e et = Some ec ->
+          wf_ec (evc e et).
+        Proof.
+          intros.
+          generalizeEverythingElse ec.
+          induction ec; intros.
+          -
+            assert (et = mt).
+            eapply inv_recon_mt; eauto.
+            subst.
+            repeat ff.
+            econstructor.
+            tauto.
+        Admitted.
+
+        eapply wf_recon; eauto.
+        
+      }
+      congruence.
+    }
+    congruence.
+  -
+    ff.
+    subst.
+    assert (et = hh n e).
+    { eapply inv_recon_hh; eauto.
+    }
+    subst.
+    repeat ff.
+  -
+    ff.
+    assert (exists et1 et2, et = ss et1 et2).
+    { eapply inv_recon_ss; eauto. }
+    destruct_conjs.
+    subst.
+    repeat ff.
+
+    assert (e = (Impl_appraisal.build_app_comp_evC e1))
+           by eauto.
+
+    assert (e0 = (Impl_appraisal.build_app_comp_evC e2))
+      by eauto.
+    
+    congruence.
+  -
+    ff.
+    assert (exists et1 et2, et = pp et1 et2).
+    { eapply inv_recon_pp; eauto. }
+    destruct_conjs.
+    subst.
+    repeat ff.
+
+    assert (e = (Impl_appraisal.build_app_comp_evC e1))
+           by eauto.
+
+    assert (e0 = (Impl_appraisal.build_app_comp_evC e2))
+      by eauto.
+    
+    congruence.
+Defined.
+
+
+(*
+    well_formed_r t ->
+    wf_ec ee ->
+    Some e' = (reconstruct_ev ecc) ->
+    copland_compile t
+                    {| st_ev := ee; st_trace := tr; st_pl := p |} =
+    (Some tt, {| st_ev := ecc;
+                 st_trace := tr';
+                 st_pl := p' |}) ->
+
+    measEvent t p (get_et ee) ev ->
+    appEvent_EvidenceC ev (build_app_comp_evC e').
+*)
